Bedrock/Platform/Facade/examples/TuplesF.v
@@ -1,0 +1,84 @@
+(** Multisets of tuples *)
+
+Require Import Bedrock Ensembles Relations.
+
+(* This section copied from Fiat for convenience, to avoid circular dependencies across libraries! *)
+Section IndexedEnsembles.
+  Context {ElementType : Type}.
+
+  Record IndexedElement :=
+    { elementIndex : nat;
+      indexedElement : ElementType }.
+
+  Definition IndexedEnsemble := Ensemble IndexedElement.
+
+  Definition IndexedEnsemble_In
+             (ensemble : IndexedEnsemble)
+             (item : ElementType) :=
+    exists idx, Ensembles.In _ ensemble {| elementIndex := idx; indexedElement := item |}.
+
+  Definition IndexedEnsembleSubtract
+             (element : ElementType)
+             (ens : IndexedEnsemble)
+  : IndexedEnsemble :=
+    fun element' => indexedElement element' <> element /\ ens element'.
+
+  (* 'Deleting' a set of tuples [R] from a relation [F] is the same
+   as taking the intersection of [F] and the complement of [R]. *)
+  Definition EnsembleDelete
+             (F : IndexedEnsemble)
+             (R : Ensemble ElementType)
+    := Intersection _ F (Complement _ (fun iel => R (indexedElement iel))).
+
+  Definition IndexedEnsembleUpdate
+             (ens : IndexedEnsemble)
+             (cond : Ensemble ElementType)
+             (updateR : relation ElementType)
+  : IndexedEnsemble
+    := fun e => (exists f: IndexedElement, ((ens f) /\ cond (indexedElement f) /\ updateR (indexedElement f) (indexedElement e))
+                                           /\ elementIndex e = elementIndex f) \/
+                ((ens e) /\ Complement _ (fun f => cond (indexedElement f)) e).
+
+  Definition UnIndexedEnsembleListEquivalence
+             (ensemble : IndexedEnsemble)
+             (l : list ElementType)  :=
+    exists l', (map indexedElement l') = l /\
+               (forall x, Ensembles.In _ ensemble x <-> List.In x l') /\
+               NoDup (map elementIndex l').
+
+  Definition UnConstrFreshIdx
+             (ensemble : IndexedEnsemble)
+             (bound : nat) :=
+  forall element,
+    ensemble element
+    -> lt (elementIndex element) bound.
+
+  Definition EnsembleIndexedListEquivalence
+             (ensemble : IndexedEnsemble)
+             (l : list ElementType) :=
+    (exists bound, UnConstrFreshIdx ensemble bound)
+    /\ UnIndexedEnsembleListEquivalence ensemble l.
+End IndexedEnsembles.
+
+Definition tuple := list W.
+Definition tuples := @IndexedEnsemble tuple.
+
+Definition EnsembleInsert {A : Type}
+           (a : A)
+           (R : Ensemble A)
+           (a' : A) :=
+  a' = a \/ R a'.
+
+Lemma in_ensemble_insert_iff :
+  forall {A} table tup inserted,
+    In A (EnsembleInsert inserted table) tup <->
+    tup = inserted \/ In A table tup.
+Proof.
+  firstorder.
+Qed.
+
+Definition insert (ts : tuples) (t : tuple) (ts' : tuples) : Prop :=
+  exists idx,
+    (forall t', In _ ts t' -> elementIndex t' <> idx)
+    /\ ts' = EnsembleInsert {| elementIndex := idx;
+                               indexedElement:= t |} ts.
